proof_of_soundness/Theorems.v
@@ -1,11 +1,3 @@
-(* IDEA:
-   First practice JUST transforming the F by adding the new function definitions to it.
-   It may be better to instead of directly adding new definitions to F, to collect all
-   the new definitions into their own map, then update the current map with the map
-   of new function in the returned map. This would allow use to add assertions about the two
-   maps being disjoint, which would in turn allow us to prove the soundness of function
-   lookup. *)
-
 Require Import
   Coq.FSets.FMapList
   Coq.Logic.Classical_Prop
@@ -95,9 +87,9 @@ Proof.
 Qed.
 
 
-Theorem no_side_effects_no_store_change_arg_eval : forall S E G F M es S' vs,
+Theorem no_side_effects_no_store_change_evalargs : forall S E G F M ps es S' vs Ef Sargs l,
   Forall (fun e => ~ ExprHasSideEffects e ) es ->
-  EvalArgs S E G F M es vs S' ->
+  EvalArgs S E G F M ps es vs S' Ef Sargs l ->
   NatMap.Equal S S'.
 Proof.
   intros. induction H0.
@@ -107,9 +99,9 @@ Proof.
 Qed.
 
 
-Theorem no_side_effects_no_store_change_arg_eval_eq : forall S E G F M es S' vs,
+Theorem no_side_effects_no_store_change_evalargs_eq : forall S E G F M ps es S' vs Ef Sargs l,
   Forall (fun e => ~ ExprHasSideEffects e ) es ->
-  EvalArgs S E G F M es vs S' ->
+  EvalArgs S E G F M ps es vs S' Ef Sargs l ->
   S = S'.
 Proof.
   intros. induction H0.
@@ -119,24 +111,29 @@ Proof.
 Qed.
 
 
-Lemma no_side_effects_evalargs_evalargs: forall S E G F M es S' vs,
+Lemma no_side_effects_evalargs_evalargs: forall S E G F M ps es S' vs Ef Sargs l,
   Forall (fun e => ~ ExprHasSideEffects e ) es ->
-  EvalArgs S E G F M es vs S' ->
-  EvalArgs S E G F M es vs S.
+  EvalArgs S E G F M ps es vs S' Ef Sargs l ->
+  EvalArgs S E G F M ps es vs S Ef Sargs l.
 Proof.
   intros. induction H0.
-  - apply EvalArgs_nil. assumption.
-  - inversion H; subst. apply EvalArgs_cons with Snext.
-    + assumption.
-    + apply no_side_effects_no_store_change_eq in H0; subst.
-      * apply IHEvalArgs. assumption.
-      * assumption.
+  - apply EvalArgs_nil.
+  - inversion H; subst. apply EvalArgs_cons with Snext; auto.
+    + apply no_side_effects_no_store_change_eq in H0; subst; auto.
 Qed.
 
 
 Lemma skip_no_side_effects : forall S E G F M S',
   EvalStmt S E G F M Skip S' ->
   NatMap.Equal S S'.
+Proof.
+  intros. induction H. reflexivity.
+Qed.
+
+
+Lemma skip_no_side_effects_eq : forall S E G F M S',
+  EvalStmt S E G F M Skip S' ->
+  S = S'.
 Proof.
   intros. induction H. reflexivity.
 Qed.
@@ -205,10 +202,10 @@ Proof.
         ~ StringMap.In x F ->
         EvalStmt S E G (StringMap.add x fdef F) M stmt S' )
       (* EvalArgs *)
-      (fun Sprev Ecaller G F M es vs Snext (h : EvalArgs Sprev Ecaller G F M es vs Snext) =>
+      (fun Sprev Ecaller G F M ps es vs Snext Ef Sargs l (h : EvalArgs Sprev Ecaller G F M ps es vs Snext Ef Sargs l) =>
         forall x fdef,
         ~ StringMap.In x F ->
-        EvalArgs Sprev Ecaller G (StringMap.add x fdef F) M es vs Snext)
+        EvalArgs Sprev Ecaller G (StringMap.add x fdef F) M ps es vs Snext Ef Sargs l)
     ); intros; try constructor; auto.
   - apply E_LocalVar with l; auto.
   - apply E_GlobalVar with l; auto.
@@ -216,12 +213,12 @@ Proof.
   - apply E_Assign_Local with l S'; auto.
   - apply E_Assign_Global with l S'; auto.
   - apply E_FunctionCall with
-      params fstmt fexpr ls Ef Sargs S' S'' S''' S'''' vs; auto.
+      params fstmt fexpr ls Ef Sargs S' S'' S''' S'''' vs l; auto.
     + apply StringMapFacts.add_mapsto_iff. right. split.
       * unfold not; intros. subst. apply StringMap_mapsto_in in m.
         contradiction.
       * auto.
-  - apply E_MacroInvocation with params mexpr M' MP ef; auto.
+  - apply E_MacroInvocation with params mexpr M' ef; auto.
   - apply EvalArgs_cons with Snext; auto.
 Qed.
 
@@ -245,10 +242,10 @@ Proof.
           StringMapProperties.Disjoint F F' ->
           EvalStmt S E G (StringMapProperties.update F F') M stmt S' )
       (* EvalArgs *)
-      (fun Sprev Ecaller G F M es vs Snext (h : EvalArgs Sprev Ecaller G F M es vs Snext) =>
+      (fun Sprev Ecaller G F M ps es vs Snext Ef Sargs l (h : EvalArgs Sprev Ecaller G F M ps es vs Snext Ef Sargs l) =>
         forall F',
           StringMapProperties.Disjoint F F' ->
-          EvalArgs Sprev Ecaller G (StringMapProperties.update F F') M es vs Snext)
+          EvalArgs Sprev Ecaller G (StringMapProperties.update F F') M ps es vs Snext Ef Sargs l)
     ); intros; try constructor; auto.
   - apply E_LocalVar with l; auto.
   - apply E_GlobalVar with l; auto.
@@ -256,7 +253,7 @@ Proof.
   - apply E_Assign_Local with l S'; auto.
   - apply E_Assign_Global with l S'; auto.
   - apply E_FunctionCall with
-      params fstmt fexpr ls Ef Sargs S' S'' S''' S'''' vs; auto.
+      params fstmt fexpr ls Ef Sargs S' S'' S''' S'''' vs l; auto.
     + apply StringMapProperties.update_mapsto_iff. right. split.
       * auto.
       * apply StringMap_mapsto_in in m.
@@ -267,16 +264,62 @@ Proof.
         apply Classical_Prop.not_and_or in H3. destruct H3.
         -- contradiction.
         -- auto.
-  - apply E_MacroInvocation with params mexpr M' MP ef; auto.
+  - apply E_MacroInvocation with params mexpr M' ef; auto.
   - apply EvalArgs_cons with Snext; auto.
 Qed.
 
 
-Lemma evalargs_notin_F_add_evalargs : forall S E G F M es vs S',
-  EvalArgs S E G F M es vs S' ->
+Lemma evalexpr_disjoint_diff_F_evalexpr : forall S E G F M e v S',
+  EvalExpr S E G F M e v S' ->
+  forall F',
+    StringMapProperties.Disjoint F F' ->
+    EvalExpr S E G (StringMapProperties.diff F F') M e v S'.
+Proof.
+  apply (
+    EvalExpr_mut
+      (* EvalExpr *)
+      (fun S E G F M e v S' (h : EvalExpr S E G F M e v S' ) =>
+        forall F',
+          StringMapProperties.Disjoint F F' ->
+          EvalExpr S E G (StringMapProperties.diff F F') M e v S' )
+      (* EvalStmt *)
+      (fun S E G F M stmt S' (h : EvalStmt S E G F M stmt S' ) =>
+        forall F',
+          StringMapProperties.Disjoint F F' ->
+          EvalStmt S E G (StringMapProperties.diff F F') M stmt S' )
+      (* EvalArgs *)
+      (fun Sprev Ecaller G F M ps es vs Snext Ef Sargs l (h : EvalArgs Sprev Ecaller G F M ps es vs Snext Ef Sargs l) =>
+        forall F',
+          StringMapProperties.Disjoint F F' ->
+          EvalArgs Sprev Ecaller G (StringMapProperties.diff F F') M ps es vs Snext Ef Sargs l)
+    ); intros; try constructor; auto.
+  - apply E_LocalVar with l; auto.
+  - apply E_GlobalVar with l; auto.
+  - apply E_BinExpr with S'; auto.
+  - apply E_Assign_Local with l S'; auto.
+  - apply E_Assign_Global with l S'; auto.
+  - apply E_FunctionCall with
+      params fstmt fexpr ls Ef Sargs S' S'' S''' S'''' vs l; auto.
+    + apply StringMapProperties.diff_mapsto_iff. split.
+      * auto.
+      * apply StringMap_mapsto_in in m.
+        unfold StringMapProperties.Disjoint in H2.
+        assert (~ (StringMap.In (elt:=function_definition) x F /\
+                    StringMap.In (elt:=function_definition) x F')).
+        { apply H2. }
+        apply Classical_Prop.not_and_or in H3. destruct H3.
+        -- contradiction.
+        -- auto.
+  - apply E_MacroInvocation with params mexpr M' ef; auto.
+  - apply EvalArgs_cons with Snext; auto.
+Qed.
+
+
+Lemma evalargs_notin_F_add_evalargs : forall S E G F M ps es vs S' Ef Sargs l,
+  EvalArgs S E G F M ps es vs S' Ef Sargs l->
   forall x fdef,
     ~ StringMap.In x F ->
-    EvalArgs S E G (StringMap.add x fdef F) M es vs S'.
+    EvalArgs S E G (StringMap.add x fdef F) M ps es vs S' Ef Sargs l.
 Proof.
   apply (
     EvalArgs_mut
@@ -291,31 +334,31 @@ Proof.
         ~ StringMap.In x F ->
         EvalStmt S E G (StringMap.add x fdef F) M stmt S' )
       (* EvalArgs *)
-      (fun Sprev Ecaller G F M es vs Snext (h : EvalArgs Sprev Ecaller G F M es vs Snext) =>
+      (fun Sprev Ecaller G F M ps es vs Snext Ef Sargs l (h : EvalArgs Sprev Ecaller G F M ps es vs Snext Ef Sargs l) =>
         forall x fdef,
         ~ StringMap.In x F ->
-        EvalArgs Sprev Ecaller G (StringMap.add x fdef F) M es vs Snext)
+        EvalArgs Sprev Ecaller G (StringMap.add x fdef F) M ps es vs Snext Ef Sargs l)
     ); intros; try constructor; auto.
   - apply E_LocalVar with l; auto.
   - apply E_GlobalVar with l; auto.
   - apply E_BinExpr with S'; auto.
   - apply E_Assign_Local with l S'; auto.
   - apply E_Assign_Global with l S'; auto.
-  - apply E_FunctionCall with params fstmt fexpr ls Ef Sargs S' S'' S''' S'''' vs; auto.
+  - apply E_FunctionCall with params fstmt fexpr ls Ef Sargs S' S'' S''' S'''' vs l; auto.
     + apply StringMapFacts.add_mapsto_iff. right. split.
       * unfold not; intros. subst. apply StringMap_mapsto_in in m.
         contradiction.
       * auto.
-  - apply E_MacroInvocation with params mexpr M' MP ef; auto.
+  - apply E_MacroInvocation with params mexpr M' ef; auto.
   - apply EvalArgs_cons with Snext; auto.
 Qed.
 
 
-Lemma evalargs_disjoint_update_F_evalargs : forall S E G F M es vs S',
-  EvalArgs S E G F M es vs S' ->
+Lemma evalargs_disjoint_update_F_evalargs : forall S E G F M ps es vs S' Ef Sargs l,
+  EvalArgs S E G F M ps es vs S' Ef Sargs l ->
   forall F',
     StringMapProperties.Disjoint F F' ->
-    EvalArgs S E G (StringMapProperties.update F F') M es vs S'.
+    EvalArgs S E G (StringMapProperties.update F F') M ps es vs S' Ef Sargs l.
 Proof.
   apply (
     EvalArgs_mut
@@ -330,17 +373,18 @@ Proof.
           StringMapProperties.Disjoint F F' ->
           EvalStmt S E G (StringMapProperties.update F F') M stmt S' )
       (* EvalArgs *)
-      (fun Sprev Ecaller G F M es vs Snext (h : EvalArgs Sprev Ecaller G F M es vs Snext) =>
+      (fun Sprev Ecaller G F M ps es vs Snext Ef Sargs l
+      (h : EvalArgs Sprev Ecaller G F M ps es vs Snext Ef Sargs l) =>
         forall F',
           StringMapProperties.Disjoint F F' ->
-          EvalArgs Sprev Ecaller G (StringMapProperties.update F F') M es vs Snext)
+          EvalArgs Sprev Ecaller G (StringMapProperties.update F F') M ps es vs Snext Ef Sargs l)
     ); intros; try constructor; auto.
   - apply E_LocalVar with l; auto.
   - apply E_GlobalVar with l; auto.
   - apply E_BinExpr with S'; auto.
   - apply E_Assign_Local with l S'; auto.
   - apply E_Assign_Global with l S'; auto.
-  - apply E_FunctionCall with params fstmt fexpr ls Ef Sargs S' S'' S''' S'''' vs; auto.
+  - apply E_FunctionCall with params fstmt fexpr ls Ef Sargs S' S'' S''' S'''' vs l; auto.
     + apply StringMapProperties.update_mapsto_iff. right. split.
       * auto.
       * apply StringMap_mapsto_in in m.
@@ -351,154 +395,49 @@ Proof.
         apply Classical_Prop.not_and_or in H3. destruct H3.
         -- contradiction.
         -- auto.
-  - apply E_MacroInvocation with params mexpr M' MP ef; auto.
+  - apply E_MacroInvocation with params mexpr M' ef; auto.
   - apply EvalArgs_cons with Snext; auto.
 Qed.
 
 
-Theorem side_effect_free_function_no_side_effects :
-  forall S E G F M x es params fstmt fexpr ls
-         Sargs S' S'' S''' Ef S'''' S''''' v vs,
-  Forall (fun e => ~ ExprHasSideEffects e) es ->
-  ~ ExprHasSideEffects fexpr ->
-  
-  fstmt = Skip ->
-  ~ StringMap.In x M ->
-  StringMap.MapsTo x (params, fstmt, fexpr) F ->
-  NoDup params ->
-  EvalArgs S E G F M es vs S' ->
-  StringMap.Equal Ef (StringMapProperties.of_list (combine params ls)) ->
-  NatMap.Equal Sargs (NatMapProperties.of_list (combine ls vs)) ->
-  NatMapProperties.Disjoint S' Sargs ->
-  NatMap.Equal S'' (NatMapProperties.update S' Sargs) ->
-  EvalStmt S'' Ef G F M fstmt S''' ->
-  EvalExpr S''' Ef G F M fexpr v S'''' ->
-  NatMap.Equal S''''' (NatMapProperties.restrict S'''' S) ->
-  EvalExpr S E G F M (CallOrInvocation x es) v S''''' ->
-  NatMap.Equal S''''' S.
-Proof.
-  intros. subst. apply no_side_effects_no_store_change_arg_eval in H5.
-  - apply skip_no_side_effects in H10. apply no_side_effects_no_store_change in H11.
-    + assert (HS: NatMap.Equal S
-                  (NatMapProperties.restrict (NatMapProperties.update S Sargs) S)).
-      { apply NatMap_disjoint_restrict_Equal. rewrite <- H5 in H8. assumption. }
-      rewrite <- H5 in H8. rewrite H9 in H10. rewrite <- H10 in H11.
-      rewrite <- H11 in H12. rewrite <- H5 in H12.
-      rewrite <- HS in H12. assumption.
-    + assumption.
-  - assumption.
-Qed.
-
-
-Lemma forall_es_combine_forall_snd: forall A B P (ks : list A) (es : list B) pair,
-  Forall (fun e => ~ P e) es ->
-  In pair (combine ks es) ->
-  ~ P (snd pair).
-Proof.
-  intros.
-  assert (In (snd pair) (snd (split (combine ks es)))).
-  apply in_split_r. assumption. destruct pair.
-  apply in_combine_r in H0. simpl.
-  rewrite Forall_forall in H. apply H. assumption.
-Qed.
-
-
-Theorem no_side_effects_msub_no_side_effects : forall mexpr params es MP,
+Lemma no_side_effects_msub_no_side_effects : forall mexpr p e,
   ~ ExprHasSideEffects mexpr ->
-  Forall (fun e => ~ ExprHasSideEffects e) es ->
-  MP = (combine params es) ->
-  ~ ExprHasSideEffects (msub MP mexpr).
+  ~ ExprHasSideEffects e ->
+  ~ ExprHasSideEffects (msub p e mexpr).
 Proof.
-  intros.
   induction mexpr; auto.
-  - simpl. destruct lookup_macro_parameter eqn: Hfind.
-    + unfold lookup_macro_parameter in Hfind.
-      apply List.find_some in Hfind.
-      apply forall_es_combine_forall_snd with (ks:=params) (es:=es).
-      assumption. rewrite H1 in Hfind. apply Hfind.
-    + auto.
-  - simpl in *. apply Classical_Prop.not_or_and in H. destruct H.
-    apply Classical_Prop.and_not_or. split.
-    + apply IHmexpr1. assumption.
-    + apply IHmexpr2. assumption.
-  - simpl in H. contradiction.
+  - (* Var *)
+    intros. simpl in *. destruct ((p =? x)%string); auto.
+  - (* BinExpr *)
+    intros. simpl in *. apply Classical_Prop.not_or_and in H. destruct H.
+    apply Classical_Prop.and_not_or. split; auto.
+  - (* Assign *)
+    intros. simpl in *. contradiction.
 Qed.
 
 
-Theorem side_effect_free_macro_no_side_effects :
-  forall S E G F M x params es mexpr M' MP ef S' v,
-  StringMap.MapsTo x (params, mexpr) M ->
+Lemma no_side_effects_Msub_no_side_effects : forall p e mexpr ef,
   ~ ExprHasSideEffects mexpr ->
-  M' = StringMap.remove x M ->
-  NoDup params ->
-  Forall (fun e => ~ExprHasSideEffects e) es ->
-  MP = combine params es ->
-  ef = msub MP mexpr ->
-  EvalExpr S E G F M' ef v S' ->
-  EvalExpr S E G F M (CallOrInvocation x es) v S' ->
-  NatMap.Equal S S'.
+  ~ ExprHasSideEffects e ->
+    MSub p e mexpr ef ->
+  ~ ExprHasSideEffects ef.
 Proof.
-  intros.
-  apply no_side_effects_no_store_change in H6. assumption.
-  rewrite H5 in H6. apply no_side_effects_msub_no_side_effects
-    with (params:=params) (es:=es) (MP:=MP) in H0.
-  - rewrite <- H5 in H0. assumption.
-  - assumption.
-  - assumption.
+  intros. induction H1; auto.
+  simpl in *. apply Classical_Prop.not_or_and in H. destruct H.
+  apply Classical_Prop.and_not_or. auto.
 Qed.
 
 
-Example transform_side_effect_free_macro_sound :
-  forall S E G F F' M x y params es mexpr M' MP ef S0' S' (v : Z)
-         ls Sargs S'' S''' Ef S'''' S''''' v vs,
-  StringMap.MapsTo x (params, mexpr) M ->
+Theorem no_side_effects_macrosubst_no_side_effects : forall mexpr params es ef,
   ~ ExprHasSideEffects mexpr ->
-  M' = StringMap.remove x M ->
-  NoDup params ->
-
-  Forall (fun e => ~ExprHasSideEffects e) es ->
-  MP = combine params es ->
-  ef = msub MP mexpr ->
-  EvalExpr S E G F M' ef v S0' ->
-  EvalExpr S E G F M (CallOrInvocation x es) v S0' ->
-
   Forall (fun e => ~ ExprHasSideEffects e) es ->
-  ~ ExprHasSideEffects mexpr ->
-  ~ StringMap.In y M ->
-
-  (* Function name maps to some function *)
-  StringMap.MapsTo y (params, Skip, mexpr) F' ->
-  (* Parameters should all be unique *)
-  NoDup params ->
-  (* Evaluate the function's arguments *)
-  EvalArgs S E G F' M es vs S' ->
-  (* Create the function environment *)
-  StringMap.Equal Ef (StringMapProperties.of_list (combine params ls)) ->
-  (* Create a store for mapping L-values to the arguments to in the store *)
-  NatMap.Equal Sargs (NatMapProperties.of_list (combine ls vs)) ->
-  (* All the L-values used in the argument store do not appear in the original store *)
-  NatMapProperties.Disjoint S' Sargs ->
-  (* Combine the argument store into the original store *)
-  NatMap.Equal S'' (NatMapProperties.update S' Sargs) ->
-  (* Evaluate the function's body *)
-  EvalStmt S'' Ef G F' M Skip S''' ->
-  EvalExpr S''' Ef G F' M mexpr v S'''' ->
-  (* Only keep in the store the L-value mappings that were there when
-     the function was called; i.e., remove from the store all mappings
-     whose L-value is in Ef/Sargs. *)
-  NatMap.Equal S''''' (NatMapProperties.restrict S'''' S) ->
-  EvalExpr S E G F' M (CallOrInvocation y es) v S''''' ->
-  NatMap.Equal S0' S'''''.
+  MacroSubst params es mexpr ef ->
+  ~ ExprHasSideEffects ef.
 Proof.
   intros.
-  apply side_effect_free_macro_no_side_effects
-    with (params:=params) (mexpr:=mexpr) (M:=M) (M':=M') (MP:=MP) (ef:=ef) in H7;
-      try assumption.
-  apply side_effect_free_function_no_side_effects with
-    (params:=params) (fstmt:=Skip) (fexpr:=mexpr) (ls:=ls) (Sargs:=Sargs) (S':=S')
-    (S'':=S'') (S''':=S''') (Ef:=Ef) (S'''':=S'''') (vs:=vs) in H21;
-      try assumption; try reflexivity.
-  rewrite <- H7. rewrite H21. reflexivity.
+  induction H1; auto.
+  inversion H0; subst.
+  apply IHMacroSubst; eauto using no_side_effects_Msub_no_side_effects.
 Qed.
 
 
@@ -512,6 +451,34 @@ Proof.
 Qed.
 
 
+Lemma no_side_effects_expr_transform_no_side_effects : forall e,
+  ~ ExprHasSideEffects e ->
+  forall M F F' e',
+    TransformExpr M F e F' e' ->
+    ~ ExprHasSideEffects e'.
+Proof.
+  intros. induction H0; auto.
+  -
+    simpl in H. apply Classical_Prop.not_or_and in H. destruct H.
+    unfold ExprHasSideEffects. fold ExprHasSideEffects.
+    apply Classical_Prop.and_not_or. split; auto.
+Qed.
+
+
+Lemma no_side_effects_Forall_no_side_effects : forall es,
+  Forall (fun e => ~ ExprHasSideEffects e) es ->
+  forall M F F' es',
+    TransformArgs M F es F' es' ->
+  Forall (fun e => ~ ExprHasSideEffects e) es'.
+Proof.
+  intros. induction H0.
+  - auto.
+  - inversion H. subst. apply Forall_cons.
+    * apply no_side_effects_expr_transform_no_side_effects with e M F F'; auto.
+    * apply IHTransformArgs; auto.
+Qed.
+
+
 (* This proof is easy right now because we only have Skip statements *)
 Lemma evalstmt_transformargs_evalstmt : forall S E G F M stmt S' F' stmt',
   EvalStmt S E G F M stmt S' ->
@@ -522,100 +489,875 @@ Proof.
 Qed.
 
 
+Lemma evalexpr_var_x_in_E_or_G : forall S E G F M x v S',
+  EvalExpr S E G F M (Var x) v S' ->
+  StringMap.In x E \/ StringMap.In x G.
+Proof.
+  intros. inversion_clear H.
+  - left. apply StringMap_mapsto_in in H0. auto.
+  - right. apply StringMap_mapsto_in in H1. auto.
+Qed.
+
+
 Scheme TransformExpr_mut := Induction for TransformExpr Sort Prop
 with TransformArgs_mut := Induction for TransformArgs Sort Prop
 with TransformStmt_mut := Induction for TransformStmt Sort Prop.
 
 
-(* Attempt 2: Induction over the transformation with schema *)
-Theorem transform_expr_sound_mut : forall M F e F' e',
+Scheme NoMacroInvocations_mut := Induction for NoMacroInvocations Sort Prop
+with NoMacroInvocationsArgs_mut := Induction for NoMacroInvocationsArgs Sort Prop.
+
+
+Lemma nomacroinvocations_remove_nomacroinvocations : forall e F M,
+  NoMacroInvocations e F M ->
+  forall x,
+  NoMacroInvocations e F (StringMap.remove x M).
+Proof.
+  apply (NoMacroInvocations_mut
+    (fun e F M (h : NoMacroInvocations e F M) =>
+      forall x,
+      NoMacroInvocations e F (StringMap.remove x M))
+    (fun es F M (h : NoMacroInvocationsArgs es F M) =>
+      forall x,
+      NoMacroInvocationsArgs es F (StringMap.remove x M))); try constructor; auto.
+  - intros. econstructor; auto.
+    + unfold not. intros. apply StringMapFacts.remove_in_iff in H1. destruct H1.
+      contradiction.
+    + apply m.
+Qed.
+
+
+Lemma nomacroinvocations_remove_evalexpr : forall S E G F M e v S',
+  EvalExpr S E G F M e v S' ->
+  NoMacroInvocations e F M ->
+  forall x,
+  EvalExpr S E G F (StringMap.remove x M) e v S'.
+Proof.
+  apply (
+    EvalExpr_mut
+      (* EvalExpr *)
+      (fun S E G F M e v S' (h : EvalExpr S E G F M e v S') =>
+        NoMacroInvocations e F M ->
+        forall x,
+        EvalExpr S E G F (StringMap.remove x M) e v S')
+      (* EvalStmt *)
+      (fun S E G F M stmt S' (h : EvalStmt S E G F M stmt S' ) =>
+        forall (x : string),
+        EvalStmt S E G F (StringMap.remove x M) stmt S' (* TODO: Fix once more statement are added *))
+      (* EvalArgs *)
+      (fun Sprev Ecaller G F M ps es vs Snext Ef Sargs l (h : EvalArgs Sprev Ecaller G F M ps es vs Snext Ef Sargs l) =>
+        NoMacroInvocationsArgs es F M ->
+        forall x,
+        EvalArgs Sprev Ecaller G F (StringMap.remove x M) ps es vs Snext Ef Sargs l )); auto; intros; try constructor.
+  - apply E_LocalVar with l; auto.
+  - apply E_GlobalVar with l; auto.
+  - inversion_clear H0; auto.
+  - inversion_clear H0; auto.
+  - inversion_clear H1. econstructor. auto. auto.
+  - inversion_clear H0. apply E_Assign_Local with l S'; auto.
+  - inversion_clear H0. apply E_Assign_Global with l S'; auto.
+  - inversion_clear H2. apply E_FunctionCall with
+    params fstmt fexpr ls Ef Sargs S' S'' S''' S'''' vs l; auto.
+    + unfold not. intros. apply StringMapFacts.remove_in_iff in H2.
+      destruct H2. contradiction.
+    + apply H1; auto.
+      assert ( (params, fstmt, fexpr) = (params0, fstmt0, fexpr0)).
+      { apply StringMapFacts.MapsTo_fun with F x; auto. }
+      inversion_clear H2. auto.
+  - inversion_clear H0. apply StringMap_mapsto_in in m. contradiction.
+  - inversion_clear H1. econstructor; auto.
+Qed.
+
+
+Lemma nomacroinvocations_remove_evalargs : forall Sprev Ecaller G F M ps es vs Snext Ef Sargs l,
+  EvalArgs Sprev Ecaller G F M ps es vs Snext Ef Sargs l ->
+  NoMacroInvocationsArgs es F M ->
+  forall x,
+  EvalArgs Sprev Ecaller G F (StringMap.remove x M) ps es vs Snext Ef Sargs l.
+Proof.
+  apply (
+    EvalArgs_mut
+      (* EvalExpr *)
+      (fun S E G F M e v S' (h : EvalExpr S E G F M e v S') =>
+        NoMacroInvocations e F M ->
+        forall x,
+        EvalExpr S E G F (StringMap.remove x M) e v S')
+      (* EvalStmt *)
+      (fun S E G F M stmt S' (h : EvalStmt S E G F M stmt S' ) =>
+        forall (x : string),
+        EvalStmt S E G F (StringMap.remove x M) stmt S' (* TODO: Fix once more statement are added *))
+      (* EvalArgs *)
+      (fun Sprev Ecaller G F M ps es vs Snext Ef Sargs l (h : EvalArgs Sprev Ecaller G F M ps es vs Snext Ef Sargs l) =>
+        NoMacroInvocationsArgs es F M ->
+        forall x,
+        EvalArgs Sprev Ecaller G F (StringMap.remove x M) ps es vs Snext Ef Sargs l )); auto; intros; try constructor.
+  - apply E_LocalVar with l; auto.
+  - apply E_GlobalVar with l; auto.
+  - inversion_clear H0; auto.
+  - inversion_clear H0; auto.
+  - inversion_clear H1. econstructor. auto. auto.
+  - inversion_clear H0. apply E_Assign_Local with l S'; auto.
+  - inversion_clear H0. apply E_Assign_Global with l S'; auto.
+  - inversion_clear H2. apply E_FunctionCall with
+    params fstmt fexpr ls Ef Sargs S' S'' S''' S'''' vs l; auto.
+    + unfold not. intros. apply StringMapFacts.remove_in_iff in H2.
+      destruct H2. contradiction.
+    + apply H1; auto.
+      assert ( (params, fstmt, fexpr) = (params0, fstmt0, fexpr0)).
+      { apply StringMapFacts.MapsTo_fun with F x; auto. }
+      inversion_clear H2. auto.
+  - inversion_clear H0. apply StringMap_mapsto_in in m. contradiction.
+  - inversion_clear H1. econstructor; auto.
+Qed.
+
+
+Lemma nomacroinvocations_transformexpr_no_change : forall e F M,
+  NoMacroInvocations e F M ->
+  forall F' e',
+  TransformExpr M F e F' e' ->
+  e = e'.
+Proof.
+  apply (NoMacroInvocations_mut
+    (fun e F M (h : NoMacroInvocations e F M) =>
+      forall F' e',
+        TransformExpr M F e F' e' ->
+        e = e')
+    (fun es F M (h : NoMacroInvocationsArgs es F M) =>
+      forall F' es',
+        TransformArgs M F es F' es' ->
+        es = es')).
+  - intros. inversion_clear H; auto.
+  - intros. inversion_clear H; auto.
+  - intros. inversion_clear H0.
+    assert (e0 = e0'). { apply H with F'; auto. }
+    subst. auto.
+  - intros. inversion_clear H0.
+    assert (e0 = e0'). { apply H with F'; auto. }
+    subst. auto.
+  - intros. inversion_clear H1.
+    assert (e1 = e1'). { apply H with F'; auto. }
+    assert (e2 = e2'). { apply H0 with F'; auto. }
+    subst. auto.
+  - intros. inversion_clear H0.
+    assert (e0 = e'0). { apply H with F'; auto. }
+    subst; auto.
+  - intros. inversion_clear H1.
+    + assert (es = es'). { apply H with F'; auto. }
+      subst; auto.
+    + apply StringMap_mapsto_in in H2. contradiction.
+  - intros. inversion_clear H. auto.
+  - intros. inversion_clear H1.
+    assert (e = e'). { apply H with F'; auto. }
+    assert (es = es'0). { apply H0 with F'; auto. }
+    subst; auto.
+Qed.
+
+
+Lemma nomacroinvocations_transformexpr_nomacroinvocations :
+  forall M F e F' e',
+  TransformExpr M F e F' e' ->
+  NoMacroInvocations e F M ->
+  NoMacroInvocations e' F' M.
+Proof.
+  apply (TransformExpr_mut
+    (* TransformExpr *)
+    (fun M F e F' e' (h : TransformExpr M F e F' e') =>
+      NoMacroInvocations e F M ->
+      NoMacroInvocations e' F' M)
+    (* TransformArgs *)
+    (fun M F es F' es' (h : TransformArgs M F es F' es') =>
+      NoMacroInvocationsArgs es F M ->
+      NoMacroInvocationsArgs es' F' M)
+    (* TransformStmt *)
+    (fun M F stmt F' stmt' (h : TransformStmt M F stmt F' stmt') =>
+      True (* TODO: Fix this later once we add more statements *))); auto.
+  - intros. inversion_clear H0. constructor; auto.
+  - intros. inversion_clear H0. constructor; auto.
+  - intros. inversion_clear H1. constructor; auto.
+  - intros. inversion_clear H0. constructor; auto.
+  - intros. inversion_clear H2. econstructor; auto.
+    + rewrite e. apply StringMapFacts.add_mapsto_iff. left; auto.
+    + apply H1.
+      assert ((params, fstmt, fexpr) = (params0, fstmt0, fexpr0)).
+      { apply StringMapFacts.MapsTo_fun with F x; auto. }
+      inversion_clear H2. auto.
+  - intros. inversion_clear H1. apply StringMap_mapsto_in in m. contradiction.
+  - intros. inversion_clear H1. constructor; auto.
+Qed.
+
+
+
+Lemma nomacroinvocations_transformargs_nomacroinvocations : forall M F es F' es',
+  TransformArgs M F es F' es' ->
+  NoMacroInvocationsArgs es F M ->
+  NoMacroInvocationsArgs es' F' M.
+Proof.
+  apply (TransformArgs_mut
+    (* TransformExpr *)
+    (fun M F e F' e' (h : TransformExpr M F e F' e') =>
+      NoMacroInvocations e F M ->
+      NoMacroInvocations e' F' M)
+    (* TransformArgs *)
+    (fun M F es F' es' (h : TransformArgs M F es F' es') =>
+      NoMacroInvocationsArgs es F M ->
+      NoMacroInvocationsArgs es' F' M)
+    (* TransformStmt *)
+    (fun M F stmt F' stmt' (h : TransformStmt M F stmt F' stmt') =>
+      True (* TODO: Fix this later once we add more statements *))); auto.
+  - intros. inversion_clear H0. constructor; auto.
+  - intros. inversion_clear H0. constructor; auto.
+  - intros. inversion_clear H1. constructor; auto.
+  - intros. inversion_clear H0. constructor; auto.
+  - intros. inversion_clear H2. econstructor; auto.
+    + rewrite e. apply StringMapFacts.add_mapsto_iff. left; auto.
+    + apply H1.
+      assert ((params, fstmt, fexpr) = (params0, fstmt0, fexpr0)).
+      { apply StringMapFacts.MapsTo_fun with F x; auto. }
+      inversion_clear H2. auto.
+  - intros. inversion_clear H1. apply StringMap_mapsto_in in m. contradiction.
+  - intros. inversion_clear H1. constructor; auto.
+Qed.
+
+
+Lemma nomacroinvocationsargs_transformargs_no_change : forall es F M,
+  NoMacroInvocationsArgs es F M ->
+  forall F' es',
+  TransformArgs M F es F' es' ->
+  es = es'.
+Proof.
+  intros. induction H0; auto.
+  inversion_clear H.
+  assert (e=e').
+  { apply nomacroinvocations_transformexpr_no_change with F M F'; auto. }
+  assert (es=es'). { apply IHTransformArgs; auto. }
+  subst; auto.
+Qed.
+
+
+Lemma nomacroinvocations_msub_nomacroinvocations : forall mexpr F M,
+  NoMacroInvocations mexpr F M ->
+  forall e,
+  NoMacroInvocations e F M ->
+  forall p,
+  NoMacroInvocations (msub p e mexpr) F M.
+Proof.
+  intros.
+  induction H; simpl.
+  - constructor.
+  - destruct ((p =? x)%string); auto; constructor.
+  - constructor. auto.
+  - constructor. auto.
+  - constructor. auto. auto.
+  - destruct ( (p =? x)%string ).
+    + destruct e; constructor; apply IHNoMacroInvocations; auto.
+    + constructor. apply IHNoMacroInvocations; auto.
+  - apply NM_CallOrInvocation with params fstmt fexpr; auto.
+Qed.
+
+
+Lemma nomacroinvocations_Msub_nomacroinvocations : forall mexpr F M,
+  NoMacroInvocations mexpr F M ->
+  forall e,
+  NoMacroInvocations e F M ->
+  forall p ef,
+  MSub p e mexpr ef ->
+  NoMacroInvocations ef F M.
+Proof.
+  apply (NoMacroInvocations_mut
+    (fun mexpr F M (h : NoMacroInvocations mexpr F M) =>
+        forall e,
+        NoMacroInvocations e F M ->
+        forall p ef,
+        MSub p e mexpr ef ->
+        NoMacroInvocations ef F M)
+    (fun es F M (h : NoMacroInvocationsArgs es F M) =>
+        forall e,
+        NoMacroInvocations e F M ->
+        forall p es',
+        MSubList p e es es' ->
+        NoMacroInvocationsArgs es' F M)); intros; try (inversion_clear H0; constructor; auto).
+  - inversion H0.
+    + subst. auto.
+    + subst. constructor.
+  - inversion_clear H1. constructor. eapply H. apply H0. apply H2.
+  - inversion_clear H1. constructor. eapply H. apply H0. apply H2.
+  - inversion_clear H2. constructor.
+    + eapply H. apply H1. apply H3.
+    + eapply H0. apply H1. apply H4.
+  - inversion_clear H1.
+    + constructor. apply H with e p; auto.
+    + constructor. apply H with e p; auto.
+  - inversion_clear H2. apply NM_CallOrInvocation with params fstmt fexpr; auto.
+    apply H with e p; auto.
+  - inversion_clear H2. constructor.
+    + apply H with e0 p; auto.
+    + apply H0 with e0 p; auto.
+Qed.
+
+
+Lemma nomacroinvocations_msubst_nomacroinvocations : forall mexpr F M,
+  NoMacroInvocations mexpr F M ->
+  forall es,
+  NoMacroInvocationsArgs es F M ->
+  forall ps ef,
+  MacroSubst ps es mexpr ef ->
+  NoMacroInvocations ef F M.
+Proof.
+  intros. induction H1.
+  - auto.
+  - inversion_clear H0. apply IHMacroSubst; auto.
+    + subst. apply nomacroinvocations_Msub_nomacroinvocations with mexpr e p; auto.
+Qed.
+
+
+Lemma novarsinenvironment_msub_novarsinenvironment : forall mexpr E,
+  NoVarsInEnvironment mexpr E ->
+  forall e,
+  NoVarsInEnvironment e E ->
+  forall p,
+  NoVarsInEnvironment (msub p e mexpr) E.
+Proof.
+  intros.
+  induction H; try constructor; try (fold msub; apply IHNoVarsInEnvironment; auto).
+  - simpl. destruct ((p =? x)%string); auto. constructor. auto.
+  - fold msub. apply IHNoVarsInEnvironment1; auto.
+  - fold msub. apply IHNoVarsInEnvironment2; auto.
+  - simpl. destruct ( (p =? x)%string); auto.
+    + destruct e; constructor; auto.
+      inversion_clear H0; auto.
+    + constructor; auto.
+  - auto.
+  - apply H1.
+Qed.
+
+
+Scheme NoVarsInEnvironment_mut := Induction for NoVarsInEnvironment Sort Prop
+with NoVarsInEnvironmentArgs_mut := Induction for NoVarsInEnvironmentArgs Sort Prop.
+
+
+(* TODO *)
+Lemma novarsinenvironment_Msub_novarsinenvironment : forall mexpr E,
+  NoVarsInEnvironment mexpr E ->
+  forall e,
+  NoVarsInEnvironment e E ->
+  forall p ef,
+  MSub p e mexpr ef ->
+  NoVarsInEnvironment ef E.
+Proof.
+  apply (NoVarsInEnvironment_mut
+    (fun mexpr E (h : NoVarsInEnvironment mexpr E) =>
+      forall e,
+      NoVarsInEnvironment e E ->
+      forall p ef,
+      MSub p e mexpr ef ->
+      NoVarsInEnvironment ef E)
+    (fun es E (h : NoVarsInEnvironmentArgs es E) =>
+      forall e,
+      NoVarsInEnvironment e E ->
+      forall p es',
+      MSubList p e es es' ->
+      NoVarsInEnvironmentArgs es' E)); intros; try constructor; auto.
+  - inversion_clear H0; constructor.
+  - inversion H0.
+    + subst; auto.
+    + subst. constructor; auto.
+  - inversion_clear H1. constructor. eapply H; eauto.
+  - inversion_clear H1. constructor. eapply H; eauto.
+  - inversion_clear H2. constructor.
+    + eapply H; eauto.
+    + eapply H0; eauto.
+  - inversion H1. 
+    + subst. constructor. inversion H0; auto. eapply H; eauto.
+    + subst. constructor; auto. eapply H; eauto.
+  - inversion_clear H1. constructor; eauto.
+  - inversion_clear H0. constructor.
+  - inversion_clear H2. constructor.
+    + eapply H; eauto.
+    + eapply H0; eauto.
+Qed.
+
+
+Lemma novarsinenvironment_msubst_novarsinenvironment : forall mexpr E,
+  NoVarsInEnvironment mexpr E ->
+  forall es,
+  Forall (fun e => NoVarsInEnvironment e E) es ->
+  forall ps ef,
+  MacroSubst ps es mexpr ef ->
+  NoVarsInEnvironment ef E.
+Proof.
+  intros. induction H1.
+  - auto.
+  - inversion_clear H0. apply IHMacroSubst; auto.
+    apply novarsinenvironment_Msub_novarsinenvironment with mexpr e p; auto.
+Qed.
+
+
+Lemma no_side_effects_no_shared_vars_with_caller_evalargs_macrosubst_nil :
+  forall mexpr,
+  (* The macro body must not have side-effects *)
+  ~ ExprHasSideEffects mexpr ->
+  forall F M,
+  (* The macro must not contain a macro invocation *)
+  NoMacroInvocations mexpr F M->
+  forall Ecaller,
+  (* The macro body must not rely on variables from the caller's scope.
+     Global variables, however, are allowed. *)
+  NoVarsInEnvironment mexpr Ecaller ->
+  forall ef,
+  MacroSubst nil nil mexpr ef ->
+  forall S G v S''',
+  EvalExpr S Ecaller G F M ef v S''' ->
+  forall S' Ef Sargs l,
+  EvalArgs S Ecaller G F M nil nil nil S' Ef Sargs l ->
+  (* We will prove that S = S' since there are no side-effects.
+     S' and Sargs must be distinct so that we don't overwrite pre-existing
+     L-values *)
+  NatMapProperties.Disjoint S' Sargs ->
+  forall v0 S'''0,
+  EvalExpr (NatMapProperties.update S' Sargs) Ef G F M mexpr v0 S'''0 ->
+  v = v0.
+Proof.
+  intros.
+  assert ((NatMapProperties.update S' Sargs) = S'''0).
+  { apply no_side_effects_no_store_change_eq in H6; auto. }
+  rewrite H7 in *.
+  inversion H2; subst. clear H2.
+  inversion H4; subst. clear H4.
+  generalize dependent v0. 
+  induction H3; intros; try (simpl in H; contradiction).
+  -
+    inversion H6; auto.
+  -
+    apply StringMap_mapsto_in in H2. inversion_clear H1.
+    contradiction.
+  -
+    inversion_clear H6.
+    + apply StringMapFacts.empty_mapsto_iff in H7. destruct H7.
+    + assert (l = l0). { apply StringMapFacts.MapsTo_fun with G x; auto. }
+      subst l0. apply NatMapProperties.update_mapsto_iff in H9. destruct H9.
+      * apply NatMapFacts.empty_mapsto_iff in H6. destruct H6.
+      * destruct H6. apply NatMapFacts.MapsTo_fun with S l; auto.
+  -
+    simpl in H. inversion_clear H0. inversion_clear H1.
+    inversion_clear H6. auto.
+  -
+    simpl in H. inversion_clear H0. inversion_clear H1.
+    inversion_clear H6. assert (v = v1). apply IHEvalExpr; auto.
+    subst v1; auto.
+  -
+    simpl in H. apply Classical_Prop.not_or_and in H. destruct H.
+    inversion_clear H0. inversion_clear H1. inversion_clear H6.
+    assert (S = S'). { apply no_side_effects_no_store_change_eq in H3_; auto. }
+    assert ((NatMapProperties.update S (NatMap.empty Z)) = S'0).
+    { apply no_side_effects_no_store_change_eq in H1; auto. }
+    subst S'. rewrite H9 in *. clear H9.
+    assert (v1 = v3). { apply IHEvalExpr1; auto. }
+    assert (v2 = v4). { apply IHEvalExpr2; auto. }
+    subst v3 v4; auto.
+Qed.
+
+
+Lemma MSub_num_num : forall p e z ef,
+  MSub p e (Num z) ef ->
+  ef = Num z.
+Proof.
+  intros. inversion H; auto. Qed.
+
+
+Lemma macrosubst_num_num : forall ps es z ef,
+  MacroSubst ps es (Num z) ef ->
+  ef = Num z.
+Proof.
+  intros. remember (Num z) as e. induction H; subst; auto.
+  apply MSub_num_num in H. subst ef.
+  apply IHMacroSubst; auto.
+Qed.
+
+
+Inductive ExprNoNamesIn : expr -> list string -> Prop :=
+  | NNI_Num : forall z ps,
+    ExprNoNamesIn (Num z) ps
+  | NNI_Var : forall x ps,
+    ~ In x ps ->
+    ExprNoNamesIn (Var x) ps
+  | NNI_ParenExpr : forall e0 ps,
+    ExprNoNamesIn e0 ps ->
+    ExprNoNamesIn (ParenExpr e0) ps
+  | NNI_UnExpr : forall uo e0 ps,
+    ExprNoNamesIn e0 ps ->
+    ExprNoNamesIn (UnExpr uo e0) ps
+  | NNI_BinExpr : forall bo e1 e2 ps,
+    ExprNoNamesIn e1 ps ->
+    ExprNoNamesIn e2 ps ->
+    ExprNoNamesIn (BinExpr bo e1 e2) ps
+  | NNI_Assign : forall x e0 ps,
+    ~ In x ps ->
+    ExprNoNamesIn e0 ps ->
+    ExprNoNamesIn (Assign x e0) ps
+  | NNI_CallOrInvocation : forall x es ps,
+    ~ In x ps ->
+    ExprNoNamesInArgs es ps ->
+    ExprNoNamesIn (CallOrInvocation x es) ps
+with ExprNoNamesInArgs : list expr -> list string -> Prop :=
+  | NNIA_nil : forall ps,
+    ExprNoNamesInArgs nil ps
+  | NNIA_cons: forall e es ps,
+    ExprNoNamesIn e ps ->
+    ExprNoNamesInArgs (e::es) ps.
+
+
+Definition unop_eq (uo1 : unop) (uo2 : unop) : bool :=
+  match uo1 with
+  | Positive => match uo2 with
+    | Positive => true
+    | Negative => false
+    end
+
+  | Negative => match uo2 with
+    | Positive => false
+    | Negative => true
+    end
+end.
+
+
+Lemma unop_eq_refl : forall uo,
+  unop_eq uo uo = true.
+Proof.
+  intros. induction uo; auto. Qed.
+
+
+Definition binop_eq (bo1 : binop) (bo2 : binop) : bool :=
+  match bo1 with
+  | Plus => match bo2 with
+    | Plus => true
+    | Sub => false
+    | Mul => false
+    | Div => false
+  end
+
+  | Sub => match bo2 with
+    | Plus => false
+    | Sub => true
+    | Mul => false
+    | Div => false
+  end
+
+  | Mul => match bo2 with
+    | Plus => false
+    | Sub => false
+    | Mul => true
+    | Div => false
+  end
+
+  | Div => match bo2 with
+    | Plus => false
+    | Sub => false
+    | Mul => false
+    | Div => true
+  end
+end.
+
+
+(* This is just syntactically equal *)
+Fixpoint expr_equal (e1: expr) (e2: expr) : Prop :=
+  match e1 with
+  | Num z1 => match e2 with
+    | Num z2 => if (z1 =? z2)%Z then True else False
+    | _ => False
+    end
+
+  | Var x => match e2 with
+    | Var y => if (x =? y)%string then True else False
+    | _ => False
+    end
+
+  | ParenExpr e10 => match e2 with
+    | ParenExpr e20 => expr_equal e10 e20
+    | _ => False
+    end
+
+  | UnExpr uo1 e10 => match e2 with
+    | UnExpr uo2 e20 => if (unop_eq uo1 uo2)
+      then expr_equal e10 e20
+      else False
+    | _ => False
+    end
+
+  | BinExpr bo1 e11 e12 => match e2 with
+    | BinExpr bo2 e21 e22 => if (binop_eq bo1 bo2) then
+      expr_equal e11 e21 /\ expr_equal e12 e22
+      else False
+    | _ => False
+    end
+
+  | Assign x e10 => match e2 with
+    | Assign y e20 => if (x =? y)%string then
+      expr_equal e10 e20
+      else False
+    | _ => False
+    end
+
+  (* FIXME *)
+  | CallOrInvocation x es => False
+end.
+
+
+Lemma binop_eq_refl : forall bo,
+  binop_eq bo bo = true.
+Proof.
+  intros. induction bo; auto. Qed.
+
+
+
+Scheme MacroSubst_EvalArgs := Induction for MacroSubst Sort Prop
+with EvalArgs_MacroSubst := Induction for EvalArgs Sort Prop.
+
+
+
+Lemma no_side_effects_no_shared_vars_with_caller_evalargs_macrosubst :
+  forall mexpr,
+  (* The macro body must not have side-effects *)
+  ~ ExprHasSideEffects mexpr ->
+  forall F M,
+  (* The macro must not contain a macro invocation *)
+  NoMacroInvocations mexpr F M->
+  forall Ecaller,
+  (* The macro body must not rely on variables from the caller's scope.
+     Global variables, however, are allowed. *)
+  NoVarsInEnvironment mexpr Ecaller ->
+  forall es,
+  Forall (fun e => ~ExprHasSideEffects e) es ->
+  (* The macro arguments must not contain a macro invocation,
+     but they may contain variables from the caller's environment *)
+  NoMacroInvocationsArgs es F M ->
+  forall S G psf vs S' Ef Sargs l,
+  (* The arguments can be evaluated to create a function environment *)
+  EvalArgs S Ecaller G F M psf es vs S' Ef Sargs l ->
+  (* We will prove that S = S' since there are no side-effects.
+     S' and Sargs must be distinct so that we don't overwrite pre-existing
+     L-values *)
+  NatMapProperties.Disjoint S' Sargs ->
+  forall v S'''0,
+  (* The function body can be evaluated using call-by-value *)
+  EvalExpr (NatMapProperties.update S' Sargs) Ef G F M mexpr v S'''0 ->
+  forall psm ef,
+  (* The arguments can be substituted into the expression body *)
+  MacroSubst psm es mexpr ef ->
+  forall v0 S''',
+  (* The expression can be evaluated using call-by-name *)
+  EvalExpr S Ecaller G F M ef v0 S''' ->
+  (* The result of evaluation should be equal *)
+  v = v0.
+Proof.
+
+
+  (* Attempt 4: Induction over mexpr followed by case-analysis on es *)
+  induction mexpr.
+  -
+    intros. apply macrosubst_num_num in H7. subst ef.
+    inversion H6. inversion H8. subst. auto.
+  -
+    destruct es.
+    + admit.
+    + inversion_clear H1. intro. inversion_clear H1.
+      intro. inversion_clear H1. intros.
+      inversion H9. subst. inversion H1. subst.
+      induction e.
+      inversion H14. subst. apply macrosubst_num_num in H17. subst ef.
+      inversion H10. inversion H13. subst.
+
+
+  (* (* Attempt 3: Induction over vs *)
+  induction vs.
+  - admit.
+  - intros. eapply IHvs; eauto.
+    (* Gets close... *) *)
+
+
+  (* (* Attempt 2: Induction over es *)
+  induction es.
+  - (* Easy*) admit.
+  - intros. eapply IHes; eauto. inversion_clear H4.
+    inversion_clear H7.
+    (* Can't prove 3 and 4 *) *)
+  
+
+  (*
+  (* Attempt 1: Induction over the argument evaluation *)
+  intros until l. intro. assert (S=S').
+  { apply no_side_effects_no_store_change_evalargs_eq in H4; auto. }
+  subst S'.
+  
+  induction H4.
+  - intros. (* Should be easy *) admit.
+  - intros. apply IHEvalArgs with S'''0 psm ef S'''; auto.
+
+  intros until ef. intros H4. induction H4.
+  - intros. apply no_side_effects_no_shared_vars_with_caller_evalargs_macrosubst_nil with
+    mexpr F M Ecaller mexpr S G S''' S' Ef Sargs l S'''0; auto.
+    + constructor.
+    + inversion H5. subst. auto.
+  (* TODO: Induction on e and mexpr? I think that could work... *)
+  - inversion_clear H2. induction e, mexpr;
+    try (simpl in H6; contradiction); try (simpl in H; contradiction).
+    + admit.
+    + admit. *)
+Abort.
+
+
+Theorem transform_expr_sound_mut_v_s : forall M F e F' e',
   TransformExpr M F e F' e' ->
   (* The proof will not work if these variables were introduced sooner.
      Doing so would interfere with the induction hypothesis *)
-  forall S E G v S',
-    EvalExpr S E G F M e v S' ->
-    EvalExpr S E G F' M e' v S'.
+  forall S E G v1 v2 S'1 S'2,
+    EvalExpr S E G F M e v1 S'1 ->
+    EvalExpr S E G F' M e' v2 S'2 ->
+    v1 = v2 /\ S'1 = S'2.
 Proof.
-  intros M F e F' e' H. apply (TransformExpr_mut
+  apply (TransformExpr_mut
     (* TransformExpr *)
     (fun M F e F' e' (h : TransformExpr M F e F' e') =>
-    forall S E G v S',
-      EvalExpr S E G F M e v S' ->
-      EvalExpr S E G F' M e' v S')
+    forall S E G v1 v2 S'1 S'2,
+      EvalExpr S E G F M e v1 S'1 ->
+      EvalExpr S E G F' M e' v2 S'2 ->
+      v1 = v2 /\ S'1 = S'2)
     (* TransformArgs *)
     (fun M F es F' es' (h : TransformArgs M F es F' es') =>
-    forall S Ecaller G vs S',
-      EvalArgs S Ecaller G F M es vs S' ->
-      EvalArgs S Ecaller G F' M es' vs S')
+    forall S Ecaller G ps1 vs1 vs2 S'1 S'2 Ef1 Ef2 Sargs1 Sargs2 l1 l2,
+      EvalArgs S Ecaller G F M ps1 es vs1 S'1 Ef1 Sargs1 l1 ->
+      EvalArgs S Ecaller G F' M ps1 es' vs2 S'2 Ef2 Sargs2 l2 ->
+      l1 = l2 /\ Ef1 = Ef2 /\ Sargs1 = Sargs2 /\ vs1 = vs2 /\ S'1 = S'2)
     (* TransformStmt *)
     (fun M F stmt F' stmt' (h : TransformStmt M F stmt F' stmt') =>
-    forall S E G S',
-      EvalStmt S E G F M stmt S' ->
-      EvalStmt S E G F' M stmt' S')); auto.
-  - intros. inversion_clear H1. apply E_ParenExpr. apply H0; auto.
-  - intros. inversion_clear H1. apply E_UnExpr. apply H0; auto.
-  - intros. inversion_clear H2. apply E_BinExpr with S'0.
-    + subst. apply evalexpr_disjoint_update_F_evalexpr; auto.
-    + subst. apply H1. apply evalexpr_disjoint_update_F_evalexpr. auto. auto.
-  - intros. inversion_clear H1.
-    + apply E_Assign_Local with l S'0; auto.
-    + apply E_Assign_Global with l S'0; auto.
-  - intros. inversion_clear H3.
-    + apply StringMapFacts.find_mapsto_iff in m.
-      apply StringMapFacts.find_mapsto_iff in H5.
-      rewrite H5 in *. inversion m. subst. clear m.
-      apply E_FunctionCall with params fstmt' fexpr' ls Ef Sargs S'0 S'' S''' S'''' vs; auto.
-      * apply StringMapFacts.add_mapsto_iff. left; auto.
-      * apply evalargs_notin_F_add_evalargs; auto.
-        apply evalargs_disjoint_update_F_evalargs; auto.
-        apply evalargs_disjoint_update_F_evalargs; auto.
-      * apply evalstmt_notin_F_add_evalstmt; auto.
-        apply evalstmt_disjoint_update_F_evalstmt; auto.
-        apply H1.
-        apply evalstmt_disjoint_update_F_evalstmt; auto.
-      * apply evalexpr_notin_F_add_evalexpr; auto.
-        apply H2.
-        apply evalexpr_disjoint_update_F_evalexpr; auto.
-        apply evalexpr_disjoint_update_F_evalexpr; auto.
+    forall S E G S'1 S'2,
+      EvalStmt S E G F M stmt S'1 ->
+      EvalStmt S E G F' M stmt' S'2 ->
+      S'1 = S'2
+      )); intros; auto.
+  -
+    inversion H. inversion H0; subst. auto.
+  -
+    inversion H; subst.
+    + inversion H0; subst.
+      * apply StringMapFacts.find_mapsto_iff in H2, H3.
+        rewrite H3 in H2. inversion H2; subst.
+        apply NatMapFacts.find_mapsto_iff in H8, H10.
+        rewrite H10 in H8. inversion H8. auto.
+      * apply StringMap_mapsto_in in H2. contradiction.
+    + inversion H0; subst.
+      * apply StringMap_mapsto_in in H4. contradiction.
+      * apply StringMapFacts.find_mapsto_iff in H3, H5.
+        rewrite H5 in H3. inversion H3; subst.
+        apply NatMapFacts.find_mapsto_iff in H9, H12.
+        rewrite H12 in H9. inversion H9. auto.
+  -
+    inversion_clear H0. inversion_clear H1.
+    destruct H with S E G v1 v2 S'1 S'2; auto.
+  -
+    inversion_clear H0. inversion_clear H1.
+    destruct H with S E G v v0 S'1 S'2; auto.
+    subst. auto.
+  -
+    inversion_clear H1. inversion_clear H2.
+    destruct H with S E G v0 v4 S' S'0; auto.
+    subst. destruct H0 with S'0 E G v3 v5 S'1 S'2; subst; auto.
+  -
+    inversion H0; subst.
+    + inversion H1; subst.
+      * apply StringMapFacts.find_mapsto_iff in H4, H5.
+        rewrite H5 in H4. inversion H4; subst.
+        destruct H with S E G v1 v2 S' S'0; auto.
+        subst. auto.
+      * apply StringMap_mapsto_in in H4. contradiction.
+    + inversion H1; subst.
+      * apply StringMap_mapsto_in in H6. contradiction.
+      * apply StringMapFacts.find_mapsto_iff in H5, H7.
+        rewrite H7 in H5. inversion H5; subst.
+        destruct H with S E G v1 v2 S' S'0; auto.
+        subst. auto.
+  -
+    inversion_clear H2. inversion_clear H3.
+    + 
+      assert (StringMap.MapsTo x (params, fstmt', fexpr') F').
+      { subst. apply StringMapFacts.add_mapsto_iff. left. auto. }
+      apply StringMapFacts.find_mapsto_iff in H15, H3.
+      rewrite H3 in H15. inversion H15. clear H15.
+      apply StringMapFacts.find_mapsto_iff in m, H5.
+      rewrite H5 in m. inversion m.
+      subst.
+      destruct H with S E G params1 vs vs0 S' S'0 Ef Ef0 Sargs Sargs0 l l0; auto.
+      destruct H15. destruct H21. destruct H25. subst.
+      destruct H0 with (NatMapProperties.update S'0 Sargs0) Ef0 G S''' S'''0 ; auto.
+      destruct H1 with S''' Ef0 G v1 v2 S'''' S''''0; auto. subst.
+      apply NatMap_Equal_eq_iff in H14, H24. subst. auto.
+    + apply StringMap_mapsto_in in H2. contradiction.
     + apply StringMap_mapsto_in in H4. contradiction.
-  - intros. inversion_clear H1.
-    + apply StringMap_mapsto_in in m. contradiction.
-    + apply StringMapFacts.find_mapsto_iff in m.
-      apply StringMapFacts.find_mapsto_iff in H2.
-      rewrite H2 in *. inversion m. subst. clear m.
-      assert (
-        EvalArgs S E G F0 M0 es vs S' /\
-        StringMap.Equal Ef (StringMapProperties.of_list (combine params ls)) /\
-        NatMap.Equal Sargs (NatMapProperties.of_list (combine ls vs)) /\
-        NatMapProperties.Disjoint S' Sargs /\
-        NatMap.Equal S'' (NatMapProperties.update S' Sargs) /\
-        EvalStmt S'' Ef G F0 M0 Skip S''' /\
-        EvalExpr S''' Ef G F0 M0 mexpr v0 S'''' /\
-        NatMap.Equal S''''' (NatMapProperties.restrict S'''' S)
-     ). { apply a. }
-     destruct H1. destruct H3. destruct H5. destruct H6. destruct H8. destruct H9.
-     destruct H10.
-      apply E_FunctionCall with
-        (params:=params) (fstmt:=Skip) (fexpr:=mexpr) (ls:=ls)
-        (Ef:=Ef) (Sargs:=Sargs) (S':=S') (S'':=S'') (S''':=S''') (S'''':=S'''')
-        (vs:=vs); auto.
-      * apply StringMapFacts.add_mapsto_iff. left; auto.
-      * apply evalargs_notin_F_add_evalargs; auto.
-      * apply evalstmt_notin_F_add_evalstmt; auto.
-        apply evalstmt_disjoint_update_F_evalstmt; auto.
-      * apply evalexpr_notin_F_add_evalexpr; auto.
-        apply evalexpr_disjoint_update_F_evalexpr; auto.
-      *
-        (* Here is where we prove that they evaluate to the same state *)
-        assert (~ ExprHasSideEffects (msub (combine params es) mexpr)).
-        { apply no_side_effects_msub_no_side_effects with params es; auto. }
-        apply no_side_effects_no_store_change in H7; auto.
-        apply no_side_effects_no_store_change_arg_eval in H1; auto.
-        apply skip_no_side_effects in H9; auto.
-        apply no_side_effects_no_store_change in H10; auto.
-        rewrite <- H7. rewrite <- H10. rewrite <- H9. rewrite H8. rewrite <- H1.
-        apply NatMap_disjoint_restrict_Equal. rewrite H1. auto.
-  - intros. inversion_clear H2. apply EvalArgs_cons with Snext.
-    + subst. apply evalexpr_disjoint_update_F_evalexpr; auto.
-    + subst. apply H1; auto using evalargs_disjoint_update_F_evalargs.
-Qed.
+  -
+    inversion H1. inversion H2.
+    + subst. apply StringMap_mapsto_in in m. contradiction.
+    + subst. apply StringMap_mapsto_in in m. contradiction.
+    + inversion H2.
+      subst S0 E0 G0 F0 M0 x0 es0 v1 S'1.
+      subst S1 E1 G1 F1 M1 x1 es1 v2 S'''''.
+      * (* This is it *)
+        
+        (* No side-effects in function *)
+        assert (mexpr = mexpr').
+        { apply nomacroinvocations_transformexpr_no_change with F M F'; auto. }
+        subst mexpr'.
+        assert ( (params1, fstmt, fexpr) = (params, Skip, mexpr) ).
+        { apply StringMapFacts.MapsTo_fun with F' fname; auto.
+          rewrite e. apply StringMapFacts.add_mapsto_iff. left. auto. }
+        inversion H3. subst params1 fstmt fexpr. clear H3.
+        assert (Forall (fun e : expr => ~ ExprHasSideEffects e) es').
+        { apply no_side_effects_Forall_no_side_effects with
+          es M F F'; auto. }
+        assert (S = S'0).
+        { apply no_side_effects_no_store_change_evalargs_eq in H22; auto. }
+        subst S'0. apply skip_no_side_effects_eq in H27. subst S'''.
+        assert (S'' = S'''').
+        { apply no_side_effects_no_store_change_eq in H33; auto. }
+        subst S''''.
+        assert (NatMap.Equal S (NatMapProperties.restrict S'' S)).
+        { rewrite H26. apply NatMap_disjoint_restrict_Equal; auto. }
+        rewrite <- H4 in H36. apply NatMap_Equal_eq_iff in H36. rewrite H36.
+        
+        (* No side-effects in macro *)
+        assert (es = es').
+        { apply nomacroinvocationsargs_transformargs_no_change with F M F'; auto. }
+        subst es'.
+        assert ( (params, mexpr) = (params0, mexpr0) ).
+        { apply StringMapFacts.MapsTo_fun with M x; auto. }
+        symmetry in H8. inversion H8. subst params0 mexpr0. clear H8.
+        assert (~ ExprHasSideEffects ef).
+        (* TODO: Fix this; probably need to add some things as premises in transformation *)
+        { apply no_side_effects_macrosubst_no_side_effects with mexpr params es; auto. }
+        assert (S = S').
+        { apply no_side_effects_no_store_change_eq in H16; auto; auto. }
+        subst S'. apply NatMap_Equal_eq_iff in H4.
+        assert (NoVarsInEnvironment mexpr E).
+        { apply n2 with S G v S; auto. }
+        split.
+        -- admit.
+        -- auto.
+        
+        (* Issues:
+           1) Proving value equivalence
+           2) Coq doesn't treatin FMap.Equal as the same thing as Logic.eq
+           
+           Solutions:
+           1) ???
+           2) Just use an axiom stating that Equal implies eq. *) 
+        
+        
+      * apply StringMap_mapsto_in in H19. contradiction. 
+  - inversion H. inversion H0. subst. split; auto.
+  - inversion H1. inversion H2.
+    destruct H with S Ecaller G v v0 Snext Snext0; auto. subst. inversion H31. subst.
+    destruct H0 with Snext0 Ecaller G ps vs vs0 S'1 S'2 Ef' Ef'0 Sargs' Sargs'0 l l0; auto.
+    destruct H4. destruct H8. destruct H9. subst.
+    split; auto.
+  - inversion H. inversion H0. subst. auto.
+Abort.
+
+
