proof_of_soundness/Transformations.v
@@ -28,104 +28,82 @@ Inductive TransformExpr :
     TransformExpr M F e0 F' e0' ->
     TransformExpr M F (UnExpr uo e0) F' (UnExpr uo e0')
   
-  | Transform_BinExpr : forall M F e1 e2 F1result F2result e1' e2' bo F' F'',
+  | Transform_BinExpr : forall bo M F e1 e2 F' e1' e2',
   
     (* Transform the left operand *)
-    StringMapProperties.Disjoint F F1result ->
-    F' = StringMapProperties.update F F1result ->
     TransformExpr M F e1 F' e1' ->
-  
+
     (* Transform the right operand *)
-    StringMapProperties.Disjoint F' F2result ->
-    F'' = StringMapProperties.update F' F2result ->
-    TransformExpr M F' e2 F'' e2' ->
-  
-    TransformExpr M F (BinExpr bo e1 e2) F'' (BinExpr bo e1' e2')
+    TransformExpr M F e2 F' e2' ->
+
+    (* This is interesting - In order for the proof to succeed, we must assert that
+     both the left and right transformations result in ultimately the same function
+     table. This is what we do in our unification step.
+     This looks funny, but it makes sense when we consider the fact that our
+     transformation is defined in "big-step" notation - that is, we are not concerned
+     with the intermediate results, just that the final function table between these
+     two operands should be equal. If we were to define the semantics using small-step
+     notation, then we would have to transform each operand one at a time *)
+
+    TransformExpr M F (BinExpr bo e1 e2) F' (BinExpr bo e1' e2')
   
   | Transform_Assign : forall M F x e F' e',
     TransformExpr M F e F' e' ->
     TransformExpr M F (Assign x e) F' (Assign x e')
 
   | Transform_FunctionCall :
-    forall   F M x es F' F'' F''' F'''' es'
-             params fstmt fexpr fstmt' fexpr'
-             Fargsresult Fstmtresult Fexprresult fname,
-    (* Macros shadow functions, so to determine if what we are calling is a function
-       it suffices just to check that its name is not in the macro table and is in
-       the function table *)
+    forall   F M x es F' es'
+             params fstmt fexpr fstmt' fexpr',
+
     ~ StringMap.In x M ->
     StringMap.MapsTo x (params, fstmt, fexpr) F ->
     
     (* Transform function arguments *)
-    StringMapProperties.Disjoint F Fargsresult ->
-    F' = StringMapProperties.update F Fargsresult ->
     TransformArgs M F es F' es' ->
     
     (* Transform function statement *)
-    StringMapProperties.Disjoint F' Fstmtresult ->
-    F'' = StringMapProperties.update F' Fstmtresult ->
-    TransformStmt M F' fstmt F'' fstmt' ->
+    TransformStmt M F fstmt F' fstmt' ->
     
     (* Transform function return expression *)
-    StringMapProperties.Disjoint F'' Fexprresult ->
-    F''' = StringMapProperties.update F'' Fexprresult ->
-    TransformExpr M F'' fexpr F''' fexpr' ->
+    TransformExpr M F fexpr F' fexpr' ->
 
     (* Add the transformed function back to the function table under a new name *)
-    ~ StringMap.In fname M ->
-    ~ StringMap.In fname F''' ->
-    F'''' = StringMap.add fname (params, fstmt', fexpr') F''' ->
+    F' = StringMap.add x (params, fstmt', fexpr') F ->
 
-    TransformExpr M F (CallOrInvocation x es) F'''' (CallOrInvocation fname es')
+    TransformExpr M F (CallOrInvocation x es) F' (CallOrInvocation x es')
     
-  | Transform_SideEffectFreeMacro :
-    forall  F M x es F' F'' Fes' es' params mexpr fname
-            (vs : list Z) (ls : list nat) (v : Z) (Ef : environment)
-            (Sargs : store) (S' : store) (S'' : store) (S''' : store)
-            (S'''' : store) (S''''' : store),
-    (* Again, macros shadow functions, so we just have to check if the callee's name
-       is in the macro table to determine if it is a macro. *)
-    
+  | Transform_SideEffectFreeNoSharedVarsWithCallerNoNestedMacro :
+    forall F M x es F' es' params mexpr mexpr' fname,
+
     StringMap.MapsTo x (params, mexpr) M ->
     
     (* The macro does not have side-effects *)
     ~ ExprHasSideEffects mexpr ->
     Forall (fun e => ~ ExprHasSideEffects e) es ->
+
+    (* The macro does not have side-effects *)
+    NoMacroInvocations mexpr F M ->
+    (* The macro arguments can share variables with the caller environment
+       since there are no side-effects, but cannnot contain nested macros *)
+    NoMacroInvocationsArgs es F M ->
+
+    (* The macro does not share variables with the caller environment *)
+    (forall S E G v S',
+      EvalExpr S E G F M (CallOrInvocation x es) v S' ->
+      NoVarsInEnvironment mexpr E) ->
+
+    (* Transform macro body *)
+    TransformExpr M F mexpr F' mexpr' ->
     
     (* Transform macro arguments *)
-    StringMapProperties.Disjoint F Fes' ->
-    F' = StringMapProperties.update F Fes' ->
     TransformArgs M F es F' es' ->
     
     (* Add the transformed function definition to the function table *)
     ~ StringMap.In fname M ->
-    ~ StringMap.In fname F' ->
-    F'' = StringMap.add fname (params, Skip, mexpr) F' ->
+    ~ StringMap.In fname F ->
+    F' = StringMap.add fname (params, Skip, mexpr') F ->
     
-    
-    (* We need to manually add all the premises for function calls that we can't
-       intuit from the proof context alone, because macro invocation just doesn't do
-       certain things that function calls do, such as evaluating arguments in an
-       eager manner *)
-    
-    (* TODO: Fix these premises *)
-
-    (forall (S : store) (E : environment) (G : environment)
-            (vs : list Z) (ls : list nat) (v : Z) (Ef : environment)
-            (Sargs : store) (S' : store) (S'' : store) (S''' : store)
-            (S'''' : store) (S''''' : store),
-
-      EvalArgs S E G F M es vs S' /\
-      StringMap.Equal Ef (StringMapProperties.of_list (combine params ls)) /\
-      NatMap.Equal Sargs (NatMapProperties.of_list (combine ls vs)) /\
-      NatMapProperties.Disjoint S' Sargs /\
-      NatMap.Equal S'' (NatMapProperties.update S' Sargs) /\
-      EvalStmt S'' Ef G F M Skip S''' /\
-      
-      EvalExpr S''' Ef G F M mexpr v S'''' /\
-      NatMap.Equal S''''' (NatMapProperties.restrict S'''' S)) ->
-    
-    TransformExpr M F (CallOrInvocation x es) F'' (CallOrInvocation fname es')
+    TransformExpr M F (CallOrInvocation x es) F' (CallOrInvocation fname es')
 with TransformArgs :
   macro_table -> function_table -> list expr ->
   function_table -> list expr -> Prop :=
@@ -135,128 +113,18 @@ with TransformArgs :
     TransformArgs M F nil F nil
   
   (* There are arguments left to transform *)
-  | TransformArgs_Cons : forall M F e es F' F'' Fe' Fes' e' es',
+  | TransformArgs_Cons : forall M F e es F' e' es',
     (* Transform the first expression *)
-    StringMapProperties.Disjoint F Fe' ->
-    F' = StringMapProperties.update F Fe' ->
     TransformExpr M F e F' e' ->
     
     (* Transform the remaining expressions *)
-    StringMapProperties.Disjoint F' Fes' ->
-    F'' = StringMapProperties.update F' Fes' ->
-    TransformArgs M F' es F'' es' ->
+    TransformArgs M F es F' es' ->
     
-    
-    TransformArgs M F (e::es) F'' (e'::es')
+    TransformArgs M F (e::es) F' (e'::es')
 with TransformStmt :
   macro_table -> function_table -> stmt ->
   function_table -> stmt -> Prop :=
   
   | Transform_Skip : forall M F,
     TransformStmt M F Skip F Skip.
-
-
-
-Inductive StepTransformExpr :
-  macro_table -> function_table -> expr ->
-  function_table -> expr -> Prop :=
-  
-  | StepTransform_Var : forall M F x,
-    StepTransformExpr M F (Var x) F (Var x)
-  
-  | StepTransform_ParenExpr : forall M F e0 F' e0',
-    StepTransformExpr M F e0 F' e0' ->
-    StepTransformExpr M F (ParenExpr e0) F' (ParenExpr e0')
-  
-  | StepTransform_UnExpr : forall M F e0 F' e0' uo,
-    StepTransformExpr M F e0 F' e0' ->
-    StepTransformExpr M F (UnExpr uo e0) F' (UnExpr uo e0')
-  
-  
-  | StepTransform_BinExprConst : forall M F bo z1 z2,
-    StepTransformExpr M F (BinExpr bo (Num z1) (Num z2)) F (BinExpr bo (Num z1) (Num z2))
-  | StepTransform_BinExpr1 : forall M F bo e1 e2 e1' F',
-    StepTransformExpr M F e1 F' e1' ->
-    StepTransformExpr M F (BinExpr bo e1 e2) F' (BinExpr bo e1' e2)
-  | StepTransform_BinExpr2 : forall M F bo z1 e2 e2' F',
-    StepTransformExpr M F e2 F' e2' ->
-    StepTransformExpr M F (BinExpr bo (Num z1) e2) F' (BinExpr bo (Num z1) e2')
-  
-  | StepTransform_Assign : forall M F x e0 F' e0',
-    StepTransformExpr M F e0 F' e0' ->
-    StepTransformExpr M F (Assign x e0) F' (Assign x e0')
-  
-  | StepTransform_Call : forall M F x es F' es',
-    StepTransformArgs M F es F' es' ->
-    StepTransformExpr M F (CallOrInvocation x es) F (CallOrInvocation x es')
-  
-with StepTransformStmt :
-  macro_table -> function_table -> stmt ->
-  function_table -> stmt -> Prop :=
-  
-  | StepTransformSkip : forall M F,
-    StepTransformStmt M F Skip F Skip
-  
-with StepTransformArgs :
-  macro_table -> function_table -> list expr ->
-  function_table -> list expr -> Prop :=
-  | StepTransformArgsNil : forall M F,
-    StepTransformArgs M F nil F nil
-  | StepTransformArgsCons : forall M F e es F' F'' e' es',
-    StepTransformExpr M F e F' e' ->
-    StepTransformArgs M F' es F'' es' ->
-    StepTransformArgs M F (e::es) F'' (e'::es').
-
-
-Scheme StepTransformExpr_mut := Induction for StepTransformExpr Sort Prop
-with StepTransformArgs_mut := Induction for StepTransformArgs Sort Prop.
-
-
-Lemma StepTransformExpr_StepExpr_StepExpr : forall M F e0 F' e1,
-  StepTransformExpr M F e0 F' e1 ->
-  forall S E G e' S',
-    StepExpr S E G F M e0 e' S' ->
-    StepExpr S E G F' M e1 e' S'.
-Proof.
-
-  intros.
-  apply (
-    StepTransformExpr_mut
-      (fun M F e0 F' e1 (h : StepTransformExpr M F e0 F' e1) =>
-        forall S E G e' S',
-          StepExpr S E G F M e0 e' S' ->
-          StepExpr S E G F M e1 e' S')
-      (fun M F es F' es' (h : StepTransformArgs M F es F' es') =>
-        forall S E G F M S' fexpr fexpr' ps,
-          StepArgs S E G F M fexpr ps es fexpr' S' ->
-          StepArgs S E G F M fexpr ps es' fexpr' S')
-    ) with e0 F; auto.
-  - intros. inversion H2; subst.
-    + inversion s.
-    + apply Step_ParenExpr1. apply H1. auto.
-  - intros. inversion H2; subst.
-    + inversion s; subst.
-    + constructor. apply H1. auto.
-  - intros. inversion H2; subst.
-    + inversion s; subst.
-    + apply Step_BinExpr1; auto.
-    + inversion s.
-  - intros. inversion H2; subst.
-    + inversion s.
-    + inversion H13.
-    + apply Step_BinExpr2. apply H1. auto.
-  - intros. inversion H2; subst.
-    + inversion s.
-    + inversion s.
-    + apply Step_Assign1. apply H1. auto.
-  - intros. inversion H2; subst.
-    apply Step_FunctionCall with params fstmt fexpr; auto.
-  - intros. admit.
-  - admit.
-  - admit.
-Abort.
-
-
-
-
 
